Observations/Measures.v
@@ -1,0 +1,70 @@
+(* Measures as integrators, a la diFinetti/Shan *)
+
+Require Import LiftedTypes.
+Require Import Weights.
+Require Import MyReals.
+
+Definition Measure (A : Type) : Type
+  := ((A -> real) -> real).
+
+(* Not every such function is a legitimate measure, but this *)
+(* characterization, along with the Lebesgue axioms below, is good *)
+(* enough for us *)
+
+(* A better version would insist that the expectation function (A -> *)
+(* Real) be measurable. *)
+
+Parameter uniform_dist : Measure real.
+
+(* The Lebesgue integral *)
+Parameter mu_L : Measure Unit.
+
+
+(* Axioms about the integral *)
+
+Axiom mu_L_const : forall (c : real) (f : Unit -> real),
+    (forall u, f u = c) -> mu_L f = c.
+
+Axiom mu_L_linear : forall c f,
+    mu_L (fun u => (times c (f u))) = (times c (mu_L f)).
+    
+Axiom split_entropy : forall f,
+    mu_L (fun u1 => mu_L (fun u2 => f u1 u2))
+    = mu_L (fun u => f (left_half u) (right_half u)).
+
+Axiom mu_L_extensional : forall f g,
+    (forall u, f u = g u) -> mu_L f = mu_L g.
+
+Lemma strict0_mu_L : forall {X : Type} (m : lifted X) h,
+    mu_L (fun u => strict0 m (fun x => h x u))
+    =
+    strict0 m (fun x => mu_L (fun u => h x u)).
+Proof.
+  destruct m; simpl; auto.
+  rewrite (mu_L_const zero); auto.
+Qed.
+
+(* An arbitrary family of real-valued measure, indexed by the reals
+   and drawn from by 'distval'.  The first argument p is the index.
+   Think of (mu_1 p) as (normal p 1.0) *)
+
+
+Parameter mu_1 : real -> Measure real.
+Parameter density_1 : real -> real -> Weight.
+
+Axiom mu_1_density_1 :
+  forall (p: real)(k : real -> real),
+    mu_1 p k = mu_L (fun u =>
+                     (times (density_1 p (unit_real u)) (k (unit_real u)))).
+
+Lemma strict20_mu_L : forall {A W : Type} (m : lifted (A * W)) h,
+    mu_L (fun u => strict20 m (fun x w => h x w u))
+    =
+    strict20 m (fun x w => mu_L (fun u => (h x w u))).
+Proof.
+  destruct m; simpl; auto.
+  rewrite (mu_L_const zero); auto.
+  destruct p; auto.
+Qed.
+
+
