Observations/OperationalSemantics.v
@@ -1,0 +1,101 @@
+(* The Operational Semantics *)
+
+Require Import Coq.Lists.List.
+Require Import Coq.Logic.FunctionalExtensionality.
+Require Import Program.
+
+Require Import EqNat. 
+
+Require Import LiftedTypes.
+Require Import MyReals.
+Require Import Weights.
+Require Import Measures.
+Require Import Types.
+Require Import Syntax.
+Require Import Substitutions.
+
+Inductive ev : forall {o: Otype}, Exp nil o -> Val nil o -> Prop :=
+| ev_val : forall o (val: Val nil o), ev (valexp val) val
+| ev_prod : forall {m m'} (e1 : Exp nil (Stype m)) (e2 : Exp nil (Stype m'))
+                   v1 v2,
+    ev e1 v1
+    -> ev e2 v2
+    -> ev (prodexp e1 e2) (prodval v1 v2)
+| ev_proj1 : forall {m m'}
+                    (e : Exp nil (Stype (Prod_type m m')))
+                    v w,
+    ev e (prodval v w) -> ev (proj1exp e) v
+                                                           
+| ev_proj2 : forall {m m'}
+                    (e : Exp nil (Stype (Prod_type m m')))
+                    v w,
+    ev e (prodval v w) -> ev (proj2exp e) w
+
+| ev_app : forall o o' (e1 : Exp nil (Funtype o o'))
+                  (e2 : Exp nil o)
+                  e' v w,
+    ev e1 (absexp e')
+    -> ev e2 v
+    -> ev (ap_Se (subst1 v) e') w
+    -> ev (appexp e1 e2) w
+| ev_bind : forall (o o': Mtype) 
+                   (e1 : Exp nil (Meastype o))
+                   (c1 : Val nil (Meastype o))
+
+                   (e2 : Exp nil (Funtype (Stype o)
+                                          (Meastype o')))
+
+                   (c2 : Val nil (Funtype (Stype o)
+                                          (Meastype o'))),
+
+    ev e1 c1 ->
+    ev e2 c2 ->
+    ev (bindexp e1 e2) (bindval c1 c2)
+| ev_return : forall o
+                     (e : Exp nil (Stype o))
+                     (c : Val nil (Stype o)),
+    ev e c ->
+    ev (returnexp e) (returnval c).
+
+(* these could be replaced by saying
+   ev_val : forall {o} (e : /etc/) ...
+ *)
+
+Arguments ev_val {_} _.
+Arguments ev_app {_ _ _ _ _ _ _} _ _ _.
+Arguments ev_bind {_ _ _ _ _} _ _ _.
+Arguments ev_return {_ _ _} _.
+
+
+
+Inductive evs : forall {o: Mtype},
+    Unit
+    -> Val nil (Meastype o)
+    -> Val nil (Stype o)
+    -> Weight
+    -> Prop :=
+| evs_unif : forall {u},
+               evs u (uniformval) (constexp (unit_real u)) one_weight
+| evs_return : forall {o u} {c: Val nil (Stype o)},
+                 evs u (returnval c) c one_weight
+| evs_bind : forall {u a b}
+                    {c1 : Val nil (Meastype a)} 
+                    {c2 : Val nil (Funtype (Stype a)(Meastype b))}
+                    {c3 c4 c5 w1 w2},
+               evs (left_half u) c1 c3 w1 ->
+               ev (appexp (valexp c2) (valexp c3)) c4 ->
+               evs (right_half u) c4 c5 w2 ->
+               evs u (bindval c1 c2) c5 (prod_weights w1 w2)
+| evs_dist : forall {p u},
+    evs u
+        (distval (constexp p))
+        (constexp (unit_real u))
+        (density_1 p (unit_real u))
+| evs_obs : forall {u p r},
+    evs u (obsval (constexp p) (constexp r)) unitval (density_1 p r).
+
+Hint Constructors ev.
+Hint Constructors evs.                    
+
+
+
