Observations/Sampling_vs_Operational.v
@@ -27,15 +27,6 @@ Ltac false_invert :=
     [ H:_ |- _ ] => solve [ inversion H ]
   end.
 
-(* Ltac helpers *)
-Ltac invert_ex :=
-  repeat
-    match goal with
-    | [ H : exists _, _ |- _ ] => inversion H; clear H; intuition
-    end.
-
-Ltac solve_ex := invert_ex; try (eexists; intuition).
-
 
 (* **************************************************************** *)
 
@@ -58,8 +49,6 @@ Function Real_Rel
   :=
     exists n, val = constexp n /\ d = n.
 
-Hint Unfold Real_Rel.
-
 Function Prod_Rel {ma mb : Mtype}
          (RA : (den_Mtype ma) -> (Val nil (Stype ma)) -> Prop)
          (RB : (den_Mtype mb) -> (Val nil (Stype mb)) -> Prop)
@@ -69,11 +58,10 @@ Function Prod_Rel {ma mb : Mtype}
     exists e1 e2, val = prodval e1 e2 /\
                   (RA (fst d) e1) /\ (RB (snd d) e2).
 
-Hint Unfold Prod_Rel.
-
 Fixpoint Mtype_Rel (m : Mtype)
   : (den_typeS (Stype m)) -> (Val nil (Stype m)) -> Prop :=
   match m with
+  | Empty_type => fun v1 v2 => True
   | Real_type => Real_Rel
   | Prod_type m1 m2 => Prod_Rel (Mtype_Rel m1) (Mtype_Rel m2) 
   end.
@@ -90,8 +78,6 @@ Function lift_Rel {o : Otype} (R : (den_typeS o) -> (Val nil o) -> Prop)
       | lift a => exists v, ev e v /\ R a v
     end.
 
-Hint Unfold lift_Rel.
-
 Definition Fun_Rel {o1 o2}
            (Rel1 : (den_typeS o1) -> (Val [] o1) -> Prop)
            (Rel2 : (lifted (den_typeS o2)) -> (Exp [] o2) -> Prop)
@@ -103,8 +89,6 @@ Definition Fun_Rel {o1 o2}
     (Rel1 a1 val2) ->
     (Rel2 (f1 a1) (ap_Se (subst1 val2) e)).
 
-Hint Unfold Fun_Rel.
-
 Definition Meas_Rel
            (m : Mtype)
            (s : den_typeS (Meastype m))
@@ -114,8 +98,6 @@ Definition Meas_Rel
       | bottom => True
       | lift (a,w) => exists c', evs u c c' w /\ Mtype_Rel m a c'
     end.
-
-Hint Unfold Meas_Rel.
 
 (* Now the main relation simply branches depending on its Otype argument: *)
 
@@ -161,7 +143,7 @@ Proof.
   apply H0.
 Qed.
 
-Hint Resolve lookup_preserves_Rel. 
+Hint Resolve lookup_preserves_Rel.
 
 Lemma extend_env_preserves_Rel :
   forall (o: Otype) G r (s : Subst G nil) (d : den_typeS o) (val: Val nil o),
@@ -175,9 +157,6 @@ Proof.
   apply H.
 Qed.
 
-Hint Resolve extend_env_preserves_Rel.
-
-    
 Lemma bind_preserves_Rel :
   forall m m'
          (s1 : den_typeS (Meastype m))
@@ -248,7 +227,7 @@ Proof.
   apply Red3b.
 Qed.
 
-Hint Resolve bind_preserves_Rel. 
+Hint Resolve bind_preserves_Rel.
 
 Lemma bind_preserves_Rel' :
   forall m m'
@@ -313,9 +292,23 @@ Proof.
 
   subst.
   eauto using evs_bind, ev_app, ev_val.
+
+  (* split. *)
+  (* eapply evs_bind. *)
+  (* eassumption. *)
+
+  (* eapply ev_app. *)
+  (* subst. *)
+  (* apply ev_val. *)
+  (* apply ev_val. *)
+  (* eassumption. *)
+  (* eassumption. *)
+  (* assumption. *)
 Qed.
 
-Hint Resolve bind_preserves_Rel'.
+
+
+
 
 Lemma return_preserves_Rel :
   forall m (v : den_typeS (Stype m)) (c : Val nil (Stype m)),
@@ -365,22 +358,6 @@ Proof.
   eauto.
 Qed.
 
-Lemma dist_preserves_Rel':
-  forall d v,
-    Real_Rel d v -> Meas_Rel Real_type (distvalS d) (distval v).
-Proof.
-  intros.
-  autounfold in *.
-  invert_ex.
-  subst.
-  eexists.
-  split.
-  eapply evs_dist.
-  unfold Mtype_Rel.
-  unfold Real_Rel.
-  eauto.
-Qed.
-
 (* This should really be of the form
   forall d v, Rel d v -> Meas_Rel _ (distvalS d) (distval v)
 
@@ -408,7 +385,14 @@ Definition Fun_Thm_Val G o   (val: Val G o):=
 
 (* Tactics for proving the fundamental theorem *)
 
+(* Ltac helpers *)
+Ltac invert_ex :=
+  repeat
+    match goal with
+    | [ H : exists _, _ |- _ ] => inversion H; clear H; intuition
+    end.
 
+Ltac solve_ex := invert_ex; try (eexists; intuition).
 
 Ltac auto_specialize :=
   repeat
@@ -429,121 +413,12 @@ Ltac destruct_lift :=
     end
   end.
 
-Theorem Fund_Thm_Proof3 : forall G o exp, @Fun_Thm_Exp G o exp.
+Theorem Fund_Thm: forall G o exp, @Fun_Thm_Exp G o exp.
 Proof.
   apply (exp_val_rec Fun_Thm_Exp Fun_Thm_Val);
   unfold Fun_Thm_Exp;
   unfold Fun_Thm_Val;
   simpl; intros;
-    try (auto_specialize;
-         repeat (destruct_lift; simpl in *; auto);
-         repeat invert_ex;
-         unfold Prod_Rel, Fun_Rel in *).
-           
-
-  { (* valexp *)
-    eauto using ev_val.
-    }
-
-  { (* prodexp *)
-    solve_ex.
-    eauto using ev_prod.
-    eexists.
-    eexists.
-    eauto.
-    }
-
-  { (* proj1exp *)
-    invert_ex.
-    subst.
-    eauto using ev_proj1.
-  }
-  
-  { (* proj2exp *)
-    invert_ex.
-    subst.
-    eauto using ev_proj2.
-  } 
-
-  { (* appexp e e0 *)
-    invert_ex.
-    destruct (d0 d) eqn: d0_d; unfold lift_Rel; auto.
-    invert_ex.
-    subst.
-    auto_specialize.
-    rewrite d0_d in *.
-    apply H5 in H3; clear H5.
-    unfold lift_Rel in H3.
-    invert_ex.
-    eexists.
-    eauto using ev_app.
-    }
-
-  { (* bindexp e e0 *)
-    invert_ex.
-    subst.
-    eexists.
-    split.
-    eauto using ev_bind.
-    eauto using bind_preserves_Rel'.
-  }
-
-  { (* returnexp e *)
-    eauto using ev_return, return_preserves_Rel.
-  }
-
-  (* Now on to values: *)
-
-  { (* valexp *)   (* this is one that the header got *)
-    unfold Real_Rel.
-    eauto.
-  }
-
-  { (* prodval *)
-    unfold Prod_Rel.
-    eauto.
-  }
-
-  { (* varexp *)
-    (* eauto using lookup_preserves_Rel doesn't work here. *)
-    apply lookup_preserves_Rel.
-    eauto.
-  }
-
-  { (* absexp *)
-    unfold Fun_Rel.
-    eexists.
-    intuition.
-    replace (ap_Se (subst1 val2) (ap_Se (shift_subst s) e))
-    with (ap_Se (cons_subst val2 s) e)
-      by (rewrite <- cSS_subst1, <- ap_cSS_e; auto).
-    auto.
-  }
-
-  { (* uniformval *)
-    auto using unif_preserves_Rel.
-  }
-
-  { (* distval *)
-    auto using dist_preserves_Rel'.
-  }
-
-  { (* bindval *)
-    auto using bind_preserves_Rel'.
-  }
-
-  { (* returnval *)
-    auto using return_preserves_Rel.
-  }
-Qed.
-
-Theorem Fund_Thm_NewProof : forall G o exp, @Fun_Thm_Exp G o exp.
-Proof.
-  apply (exp_val_rec Fun_Thm_Exp Fun_Thm_Val);
-  unfold Fun_Thm_Exp;
-  unfold Fun_Thm_Val;
-  simpl; intros;
-    (* this script knocks off 5 cases *)
   try solve [auto_specialize; eauto;
                   repeat destruct_lift;
                   unfold Prod_Rel, lift_Rel in *;
@@ -562,7 +437,7 @@ Proof.
     rewrite d0_d in *.
     simpl in H4.
     invert_ex.
-    eauto using ev_app.
+    eauto.
     }
 
   (* Now on to values: *)
@@ -589,190 +464,19 @@ Proof.
     rewrite H1.
     apply dist_preserves_Rel.
     }
-Qed.
 
-
-
-
-Theorem Fund_Thm: forall G o exp, @Fun_Thm_Exp G o exp.
-Proof.
-  apply (exp_val_rec Fun_Thm_Exp Fun_Thm_Val);
-  unfold Fun_Thm_Exp;
-  unfold Fun_Thm_Val;
-  intros;
-  simpl.
-
-  (* valexp *)
-  { specialize (H _ _ H0).
-    exists (ap_Sv s v).
-    split.
-    apply ev_val.
-    apply H.
-    }
-
-  { (* prodexp e1 e2 *)
+  { (* obsval *)
+    auto_specialize.
+    unfold Real_Rel in *.
+    invert_ex.
+    unfold Meas_Rel.
     intros.
-    specialize (H _ _ H1).
-    specialize (H0 _ _ H1).
-    destruct (den_expS e r), (den_expS e0 r); simpl; auto.
-    simpl in *.
-    inversion H.
-    inversion H0.
-    exists (prodval x x0).
-    inversion H2; clear H2.
-    inversion H3; clear H3.
-    split.
-    apply ev_prod; auto.
-    unfold Prod_Rel.
-    eauto.
-  }
-
-  { (* proj1exp e *)
-    specialize (H r s H0); clear H0.
-    destruct (den_expS e r); simpl; auto.
-    inversion H. clear H. inversion H0. clear H0.
-    unfold Rel in H1.
-    simpl in H1.
-    unfold Prod_Rel in H1.
-    inversion H1; clear H1.
-    inversion H0; clear H0.
-    inversion H1; clear H1.
-    inversion H2; clear H2.
-    exists x0.
-    split.
-    apply (ev_proj1 _ x0 x1).
-    rewrite H0 in H.
-    apply H.
+    simpl.
+    exists unitval.
+    subst.
+    rewrite H0,H2.
     auto.
   }
     
- { (* proj2exp e *)
-    specialize (H r s H0); clear H0.
-    destruct (den_expS e r); simpl; auto.
-    inversion H. clear H. inversion H0. clear H0.
-    unfold Rel in H1.
-    simpl in H1.
-    unfold Prod_Rel in H1.
-    inversion H1; clear H1.
-    inversion H0; clear H0.
-    inversion H1; clear H1.
-    inversion H2; clear H2.
-    exists x1.
-    split.
-    apply (ev_proj2 _ x0 x1).
-    rewrite H0 in H.
-    apply H.
-    auto.
-  }
 
-
- { (* appexp e e0 *)
-    specialize (H _ _ H1).
-    specialize (H0 _ _ H1).
-    destruct (den_expS e r), (den_expS e0 r); simpl in *; auto.
-
-    (* work out the first reduction *)
-    inversion H; clear H; intuition.
-    inversion H0; clear H0; intuition.
-    inversion H3 as [e']; clear H3; intuition.
-    subst.
-    (* H: ev (ap_Se s e) (absexp e') *)
-    (* H0: ev (ap_Se s e0) x *)
-
-    (* now the third reduction *)
-    specialize (H5 _ _ H4).
-    destruct (d d0); simpl in *; auto.
-    inversion H5; clear H5; intuition.
-    eauto using ev_app.
-
-  }
-
-  (* bindexp e e0 *)
-  { specialize (H _ _ H1).
-    specialize (H0 _ _ H1).
-    destruct (den_expS e r), (den_expS e0 r); simpl in *; auto.
-    inversion H0; inversion H; intuition.
-    eauto using ev_bind, bind_preserves_Rel.
-  }
-
-  (* returnexp e *)
-  { specialize (H _ _ H0).
-    destruct (den_expS e r); simpl in *; auto.
-    inversion H; intuition.
-    eauto using ev_return, return_preserves_Rel.
-    }
-
-  (* constexp *)
-  { unfold coerce_realS.
-    unfold Real_Rel.
-    eauto. }
-
-  { (* prodval *)
-    specialize (H r s H1).
-    specialize (H0 r s H1).
-    unfold Prod_Rel.
-    eauto.
-    }
-
-  (* varexp  (which is a Val!) *)
-    apply lookup_preserves_Rel. assumption.
-
-  { (* absexp *)
-    unfold Fun_Rel.
-    exists (ap_Se (shift_subst s) e).
-    split; auto.
-    intros.
-
-    assert (H2: (Rel_Env (cons_env a1 r) (cons_subst val2 s))).
-    apply extend_env_preserves_Rel; auto.
-    specialize (H _ _ H2).
-
-    assert (H3: (ap_Se (cons_subst val2 s) e)
-                =
-                (ap_Se (subst1 val2) (ap_Se (shift_subst s) e))).
-    rewrite <- cSS_subst1.
-    rewrite <- ap_cSS_e.
-    auto.
-    rewrite <- H3 in *.
-    apply H.
-    }
-
-  { (* uniformval *)
-    unfold Meas_Rel.
-    intros.
-    unfold uniformopS.
-    exists (constexp (unit_real u)). (* this could be an eexists *)
-    split.
-    apply evs_unif.
-    simpl.
-    unfold Real_Rel.
-    eauto.
-  }
-
-  { (* distval *)
-    (* this should be turned into a lemma distval_preserves_Rel *)
-    specialize (H _ _ H0).
-    unfold Rel in H.
-    unfold Mtype_Rel in H.
-    unfold Real_Rel in H.
-    inversion H; clear H; intuition.
-    subst.
-    rewrite H.
-    apply dist_preserves_Rel.
-  }
-
-
-  { (* bindval *)
-    apply bind_preserves_Rel.
-    specialize (H _ _ H1).
-    specialize (H0 _ _ H1).
-    apply H.
-    specialize (H0 _ _ H1).
-    apply H0.
-  }
-
-  { (* returnval *)
-    apply return_preserves_Rel.
-    specialize (H _ _ H0).
-    apply H. }
 Qed.
