Observations/Substitutions.v
@@ -1,0 +1,398 @@
+(* Substitutions and Renamings, following Benton-Hur-Kennedy-Varming *)
+
+Require Import Coq.Lists.List.
+Require Import Coq.Logic.FunctionalExtensionality.
+Require Import Program.
+
+Require Import EqNat. 
+
+Require Import LiftedTypes.
+Require Import MyReals.
+Require Import Types.
+Require Import Syntax.
+
+
+
+(* **************** Substitutions **************** *)
+
+(* Substitutions: following Benton-Hur-Kennedy *)
+
+(* A Subst G G' is a function that takes an o, a o-valued variable in *)
+(*    G and returns an o-valued value that is  well-typed in G'  *)
+
+(* It would be nice to represent a substitution as a heterogenous list,
+   like we did for value environments, but I couldn't make this work. 
+   We will, however, use subst_lookup as an interface in most 
+   (if not all) places. *)
+
+Definition Subst G G': Type := forall o, Var G o -> Val G' o.
+
+Function subst_lookup {G G' o}
+         (var: Var G o)
+         (s : Subst G G')
+: (Val G' o)
+  :=
+    (s o var).
+
+Definition id_subst {G} : Subst G G := fun o var => varexp var.
+
+(* (cons_subst val s)(var0) = val, *)
+(* (cons_subst val s)(var_n) = s(var(n-1)) *)
+
+Program Definition cons_subst {G G' o}  (* fixpoint doesn't work here, I *)
+                                        (* don't know why *)
+         (val : Val G' o)
+         (s : Subst G G')
+: (Subst (o::G) G') :=
+  fun o' (var : Var (o::G) o') =>
+    match var with
+      | var_0 => val
+      | var_S v' => s _ v'
+    end.
+
+(*  singleton substitution [val/*1*] *)
+Function subst1 {G o} (val : Val G o) : (Subst (o::G) G) :=
+  (cons_subst val id_subst).
+
+
+Definition hd_subst {G G':Tyenv}{o}
+           (s : Subst (o::G) G')
+: Val G' o := subst_lookup var_0 s.
+
+
+Definition tl_subst {G G' o}
+           (s : Subst (o::G) G')
+: Subst G G'
+  :=
+    fun o' v => s o' (var_S v).
+
+(* **************** Renamings **************** *)
+
+(* We want to substitute inside abstractions, but we don't have enough *)
+(* operations on substitutions yet. *)
+
+(* We eventually need to deal with grotty details of deBruijn
+   shifting.  To do this, we follow BKV and introduce Renamings 
+   as a way of operating on the results of substitutions.
+*)
+
+(* A Renaming G G' is a function from variables defined over G to *)
+(* variables defined over G' *)
+
+Definition Renaming G G' := forall o, Var G o -> Var G' o.
+
+Definition id_renaming G : Renaming G G := fun o v => v.
+
+(* rename var_0 to var, others as per renaming r *)
+
+Program Definition cons_renaming {G G' o}
+        (var : Var G' o)
+        (r : Renaming G G')
+: (Renaming (o::G) G')
+   := fun o' (in_var : Var (o::G) o') =>
+        match in_var with
+          | var_0 => var
+          | var_S v' => r o' v'
+        end.
+
+(* pad_renaming: Given that we have a renaming r from G to G', 
+   renames (var_0 (o::G)) to (var_0 (o::G')), renames other variables 
+   according to r *)
+
+Program Definition pad_renaming {G G' o} (ren : Renaming G G')
+: (Renaming (o::G) (o::G'))
+  :=
+    fun o' v =>
+      match v with
+        | var_0  => var_0 
+        | var_S  v' => var_S (ren _ v')
+      end.
+
+(* apply renaming.  Our naming convention calls these ap and ap_Re *)
+
+Fixpoint ap_Rv {G G' o} (ren : Renaming G G')
+         (val : Val G o) : (Val G' o) :=
+  match val with
+  | varexp var => varexp (ren _ var)
+  | prodval v1 v2 => prodval (ap_Rv ren v1) (ap_Rv ren v2)
+  | absexp e => absexp (ap_Re (pad_renaming ren) e)
+  | constexp n => constexp n 
+  | uniformval => uniformval
+  | bindval v1 v2 => bindval (ap_Rv ren v1) (ap_Rv ren v2)
+  | obsval v1 v2 => obsval (ap_Rv ren v1) (ap_Rv ren v2)
+  | returnval v => returnval (ap_Rv ren v)
+  | distval v => distval (ap_Rv ren v)
+  | unitval => unitval
+  end
+with
+ap_Re {G G' o} (ren : Renaming G G') (exp : Exp G o)
+: (Exp G' o) :=
+  match exp with
+  | valexp val => valexp (ap_Rv ren val)
+  | prodexp e1 e2 => prodexp (ap_Re ren e1) (ap_Re ren e2)
+  | proj1exp e1 => proj1exp (ap_Re ren e1)
+  | proj2exp e1 => proj2exp (ap_Re ren e1)
+  | appexp e1 e2 => appexp (ap_Re ren e1) (ap_Re ren e2)
+  | bindexp e1 e2 => bindexp (ap_Re ren e1) (ap_Re ren e2)
+  | returnexp e1 => returnexp (ap_Re ren e1)
+  end.
+
+Hint Resolve ap_Rv ap_Re.
+
+(* GIVEN: subst : Subst G G',  *)
+(* RETURNS: a new substitution, with var0 bound to var0:o, and 
+   var(n+1) bound to (subst var(n)), with all the variables incremented by 1 *)
+
+Program Definition shift_subst {G G' o}
+        (subst : Subst G G') : (Subst (o::G) (o::G')) 
+   :=
+     fun _ var =>
+       match var with
+         | var_0 => varexp var_0
+         | var_S var' => ap_Rv  (* increment variables in the range of subst *)
+                                 (fun _ var'' => var_S var'')
+                                 (subst _ var')
+       end.
+
+(* applying a substitution to a value or exp *)
+
+Fixpoint ap_Sv {G G' o} (s : Subst G G') (val : Val G o) : (Val G' o)
+  :=
+    match val with
+    | constexp n => constexp n
+    | prodval v1 v2 => prodval (ap_Sv s v1) (ap_Sv s v2)
+      | varexp var => subst_lookup var s
+      | absexp e => absexp (ap_Se (shift_subst s) e)
+      | uniformval => @uniformval _
+      | bindval e1 e2 => bindval (ap_Sv s e1) (ap_Sv s e2)
+      | obsval e1 e2 => obsval (ap_Sv s e1) (ap_Sv s e2)
+      | returnval v => returnval (ap_Sv s v)
+      | distval v => distval (ap_Sv s v)
+      | unitval => unitval
+    end
+with
+ap_Se {G G' o} (s : Subst G G') (e : Exp G o) : (Exp G' o)
+:=
+  match e with
+  | valexp val => valexp (ap_Sv s val)
+  | prodexp e1 e2 => prodexp (ap_Se s e1) (ap_Se s e2)
+  | proj1exp e1 => proj1exp (ap_Se s e1)
+  | proj2exp e1 => proj2exp (ap_Se s e1)
+  | appexp e1 e2 => appexp (ap_Se s e1) (ap_Se s e2)
+  | bindexp  e1 e2 => bindexp (ap_Se s e1) (ap_Se s e2)
+  | returnexp e1 => returnexp (ap_Se s e1)
+  end.
+
+Hint Resolve ap_Sv ap_Se.
+
+(* compositions of renamings and substitutions.  All are right-to-left *)
+
+Definition c_RR {E E' E''} (r : Renaming E' E'') (r' : Renaming E E') := 
+  (fun t v => r t (r' t v)) : Renaming E E''.
+
+Definition c_SR {E E' E''} (s : Subst E' E'') (r : Renaming E E')  := 
+  (fun t v => s t (r  t v)) : Subst E E''.
+
+Definition c_RS {E E' E''} (r : Renaming E' E'') (s : Subst E E')  := 
+  (fun t v => ap_Rv r (s t v)) : Subst E E''.
+
+Definition c_SS {E E' E''} (s : Subst E' E'') (s' : Subst E E') := 
+  (fun t v => ap_Sv s (s' t v)) : Subst E E''.
+
+
+
+(* Tactic From BKV: applies functional_extensionality twice
+   -- useful for substitutions, which take two arguments *)
+Ltac ExtVar :=
+ match goal with
+    [ |- ?X = ?Y ] => 
+    (apply (@functional_extensionality_dep _ _ X Y) ; 
+     let t := fresh "t" in intro t;
+     apply functional_extensionality; 
+     let v := fresh "v" in intro v; 
+     dependent destruction v; auto) 
+ end.
+
+Ltac Rewrites E := 
+  (intros; simpl; try rewrite E; 
+   repeat (match goal with | [H:context[_=_] |- _] => rewrite H end); 
+   auto).
+
+
+(* **************************************************************** *)
+
+(* ***** Algebraic Properties of substitutions and renamings  ***** *)
+
+(* The object of this part of the development is to get to ap_cSS_e, which 
+   describes how application distributes over composition of substitutions. 
+   *)
+
+Lemma shift_id_subst : forall E t,
+                         shift_subst (@id_subst E) = @id_subst (t::E). 
+Proof. intros. ExtVar. Qed.
+
+Lemma ap_Sv_id :
+  forall G o (e : Val G o), ap_Sv id_subst e = e. 
+Proof.
+  apply (val_exp_rec
+           (fun E t (e : Exp E t) => ap_Se id_subst e = e)
+           (fun E t (v : Val E t) => ap_Sv id_subst v = v));
+  intros; simpl; eauto; try rewrite H; try rewrite H0; auto.
+  rewrite shift_id_subst.
+  rewrite H.
+  auto.
+Qed.
+
+(* pad distributes over composition of renamings *)
+Lemma pad_cRR : forall G G' G'' o
+                            (r : Renaming G' G'')
+                            (r' : Renaming G G'),
+                       (pad_renaming (o:=o)
+                          (c_RR r r')) =
+                       (c_RR (pad_renaming r)
+                             (pad_renaming r')).
+Proof.  intros.  ExtVar. Qed.
+
+Lemma ap_cRR_v :
+  forall G t (e: Val G t) G' G''
+         (r : Renaming G' G'')
+         (r' : Renaming G G'),
+    (ap_Rv (c_RR r r') e) =
+    (ap_Rv r (ap_Rv r' e)).
+Proof.
+  apply (val_exp_rec
+           (fun G t (e : Exp G t) =>
+              forall G' G''
+                     (r : Renaming G' G'')
+                     (r' : Renaming G G'),
+                (ap_Re (c_RR r r') e) = (ap_Re r (ap_Re r' e)))
+           (fun G t (v : Val G t) =>
+              forall G' G''
+                     (r : Renaming G' G'')
+                     (r' : Renaming G G'),
+                (ap_Rv (c_RR r r') v) = (ap_Rv r (ap_Rv r' v))));
+  Rewrites pad_cRR.
+Qed.
+
+Lemma shift_cSR :
+  forall G G' G'' o
+         (s : Subst G' G'') (r: Renaming G G'),
+    shift_subst (o:=o) (c_SR s r)
+    = c_SR (shift_subst s) (pad_renaming r).
+Proof. intros. ExtVar. Qed.
+
+Lemma ap_cSR_v : forall E t (e:Val E t) E' E''
+                        (s:Subst E' E'')
+                        (r:Renaming E E'), 
+                   ap_Sv (c_SR s r) e = ap_Sv s (ap_Rv r e).
+Proof.
+  apply (val_exp_rec
+           (fun E t (e : Exp E t) =>
+              forall  E' E''
+                      (s:Subst E' E'') (r:Renaming E E'), 
+                ap_Se (c_SR s r) e = ap_Se s (ap_Re r e))
+           (fun E t (v : Val E t) =>
+              forall  E' E''
+                      (s:Subst E' E'') (r:Renaming E E'), 
+                ap_Sv (c_SR s r) v = ap_Sv s (ap_Rv r v)));
+  (intros; Rewrites H; Rewrites shift_cSR).
+Qed.
+
+Lemma shift_cRS : forall G0 G1 G2 o
+                         (r : Renaming G1 G2)
+                         (s : Subst G0 G1),
+                    shift_subst (o:=o) (c_RS r s)
+                    = c_RS (pad_renaming r) (shift_subst s).
+Proof.
+  intros.
+  ExtVar.
+  unfold c_RS. 
+  simpl.       
+  unfold shift_subst.
+  simpl.
+  rewrite <-  2 ap_cRR_v.
+  unfold c_RR.
+  simpl.
+  reflexivity.
+Qed.
+
+Lemma ap_cRS_v : forall
+                   G o (e : Val G o) G' G''
+                   (r : Renaming G' G'')
+                   (s : Subst G G'),
+                 (ap_Sv (c_RS r s) e) = (ap_Rv r (ap_Sv s e)).
+Proof.
+  apply (val_exp_rec
+           (fun G o (e : Exp G o) =>
+              forall G' G''
+                     (r : Renaming G' G'')
+                     (s : Subst G G'),
+                (ap_Se (c_RS r s) e)
+                = (ap_Re r (ap_Se s e)))
+           (fun G o (e : Val G o) =>
+              forall G' G''
+                     (r : Renaming G' G'')
+                     (s : Subst G G'),
+                (ap_Sv (c_RS r s) e)
+                = (ap_Rv r (ap_Sv s e)))); Rewrites shift_cRS.
+Qed.
+
+
+
+Lemma shift_cSS :
+  forall G G' G'' o
+         (s: Subst G' G'')
+         (s' : Subst G G'),
+    (shift_subst (o:=o) (c_SS s s'))
+    = (c_SS (shift_subst s) (shift_subst s')).
+Proof.
+  intros.
+  ExtVar.
+  simpl.
+  unfold c_SS.
+  simpl.
+  rewrite <- ap_cRS_v.
+  rewrite <- ap_cSR_v.
+  auto.   (* not sure what this is doing here, 
+             but I'm too tired to investigate. *) 
+Qed.
+
+Lemma ap_cSS_e: forall G o (e : Exp G o) G' G''
+                       (s : Subst G' G'')
+                       (s': Subst G G'),
+                  (ap_Se (c_SS s s') e)
+                    = (ap_Se s (ap_Se s' e)).
+Proof.
+  apply (exp_val_rec
+            (fun G o (exp: Exp G o) =>
+                 forall G' G'' (s : Subst G' G'')
+                        (s': Subst G G'),
+                   (ap_Se (c_SS s s') exp)
+                   = (ap_Se s (ap_Se s' exp)))
+            (fun G o (val: Val G o) =>
+                 forall G' G'' (s : Subst G' G'')
+                        (s': Subst G G'), 
+                   (ap_Sv (c_SS s s') val)
+                   = (ap_Sv s (ap_Sv s' val))));
+  Rewrites shift_cSS.
+Qed.
+
+
+Lemma cSS_subst1 : forall G o (val : Val G o) G',
+                   forall (s : Subst G' G),
+                     (c_SS (subst1 val) (shift_subst s))
+                     = (cons_subst val s).
+Proof.
+  intros.
+  unfold c_SS.
+  ExtVar.
+  simpl.
+  rewrite <- ap_cSR_v.
+  unfold c_SR.
+  simpl.
+  assert (H0 : (fun t var => @id_subst G t var) = id_subst) by ExtVar.
+  rewrite H0.
+  rewrite ap_Sv_id.
+  reflexivity.
+Qed.
+
