Observations/Types.v
@@ -1,0 +1,90 @@
+(* types of the object language *)
+(* and environments *)
+
+Require Import Coq.Lists.List.
+
+Require Import LiftedTypes.
+Require Import Weights.
+Require Import MyReals.                   (* including times: Weight -> real -> real *)
+Require Import Measures.
+
+
+(* Measurable types *)
+
+Inductive Mtype : Type :=
+| Empty_type : Mtype
+| Real_type : Mtype
+| Prod_type : Mtype -> Mtype -> Mtype.
+
+
+(* denotations of measurable types: same for both *)
+
+Function den_Mtype (m : Mtype) : Type :=
+  match m with
+  | Empty_type => unit
+  | Real_type => real
+  | Prod_type m1 m2 => (den_Mtype m1) * (den_Mtype m2)
+  end.
+    
+(* M_Otype => Stype (Scalar type) *)
+
+(* Note that in this organization we can build products only of *)
+(* measurable types.  Can't build the product of a function type or a *)
+(* measure type and anything else.  I don't think there's anything *)
+(* significant about that, but it's beyond my Coq skills. *)
+
+Inductive Otype : Type :=
+| Stype : Mtype -> Otype        (* injection *)
+| Meastype : Mtype -> Otype    (* Meas A *)
+| Funtype : Otype -> Otype -> Otype.
+                          
+(* Environments *)
+
+Definition Tyenv := list Otype.
+
+(* den_env G is the type of value environments compatible with G *)
+
+Fixpoint den_env {den_type : Otype -> Type}(G : Tyenv) : Type :=
+  match G with
+    | nil => unit
+    | (cons o G') =>  (den_type o) * (@den_env den_type G')
+  end.
+
+Function cons_env {o}{G : Tyenv} {den_type : Otype -> Type} (d : den_type o) (r : den_env G) 
+: (den_env (o::G)) := (d, r).
+
+(* Represent variables following Benton, Kennedy, and Varming*)
+
+(* v : Var G o iff v is a variable of type o in G *)
+(* the n-th variable in (Var G o) is, roughly speaking, a proof that the
+   the n-th position in G is of type o. *)
+
+Inductive Var : Tyenv -> Otype -> Type :=
+| var_0 : forall (G : Tyenv) (o : Otype), Var (cons o G) o
+| var_S : forall G o o', Var G o -> Var (cons o' G) o.
+
+Arguments var_0 {_ _}.
+Arguments var_S {_ _ _} _.
+
+
+Fixpoint env_lookup
+         {G : Tyenv}
+         {o : Otype}
+         {den_type : Otype -> Type}
+         (v : Var G o) : (den_env G) -> (den_type o) 
+:=  match v 
+  with
+    | var_0 => fun venv => fst venv
+    | var_S v'  => fun venv => env_lookup v' (snd venv)
+    end.
+
+(* Simply reversing the arguments to env_lookup doesn't work, so
+   apply_env has to call env_lookup *)
+
+Definition apply_env
+         {G : Tyenv}
+         {o : Otype}
+         {den_type : Otype -> Type}
+         (r : den_env G)
+         (v : Var G o) : (den_type o) 
+  :=  env_lookup v r.
